\documentclass[a4paper]{exam}

\usepackage{amsmath}
\usepackage{geometry}
\usepackage{graphicx}
\usepackage{hyperref}
\usepackage{titling}

% Header and footer.
\pagestyle{headandfoot}
\runningheadrule
\runningfootrule
\runningheader{CS 212, Fall 2022}{WC 05: Ambiguity in Context-Free Grammars}{\theauthor}
\runningfooter{}{Page \thepage\ of \numpages}{}
\firstpageheader{}{}{}

\printanswers

\title{Weekly Challenge 05: Ambiguity in Context-Free Grammars}
\author{mj06879} % <=== replace with your student ID, e.g. xy012345
\date{CS 212 Nature of Computation\\Habib University\\Fall 2022}

\qformat{{\large\bf \thequestion. \thequestiontitle}\hfill}
\boxedpoints

\begin{document}
\maketitle

\begin{questions}
  
\titledquestion{Ambiguous or not?}

  Prove whether the following CFG is ambiguous or not.
  \begin{align*}
    S & \to AS \mid \epsilon\\
    A & \to BA \mid a\\
    B & \to SB \mid b\\
  \end{align*}
  
  \begin{solution}
    % Enter your solution here.
    According to Definition 2.7 of Textbook:
    \begin{center}
    ``A string $w$ is derived $\mathbf{ambiguously}$ in context-free grammar $G$ if
it has two or more different leftmost derivations. Grammar $G$ is
ambiguous if it generates some string ambiguously."
    \end{center}
Here we are doing proof by contradiction by taking string $w$ = $``\mathbf{abba}"$ that can be derived by two different leftmost derivations to show that the given CFG is ambiguous. \\
\textbf{Note:} we are not limiting that these are the only derivations for this string.\\
On left hand side of derivations we are underlining the Variable that is going to be converted.\\
\underline{\textbf{First Derivation:}}
\[ \underline{S} \to AS , \text{ \hspace{1cm} Using S $\to$ AS}\]
\[  \underline{A}S \to aS , \text{ \hspace{1cm} Using A $\to$ a}\]
\[ a \underline{S} \to aAS, \text{ \hspace{1cm} Using S $\to$ AS}\]
\[ a \underline{A}S \to aBAS,  \text{ \hspace{1cm} Using A $\to$ BA}\]
\[ a \underline{B}AS \to abAS, \text{ \hspace{1cm} Using B $\to$ b} \]
\[ ab \underline{A}S \to abBAS, \text{\hspace{1cm} Using A $\to$ BA} \]
\[ ab \underline{B}AS  \to abbAS, \text{ \hspace{1cm} Using B $\to$ b}\]
\[ abb \underline{A}S \to abbaS , \text{ \hspace{1cm} Using A $\to$ a}\]
\[ abba \underline{S} \to abba  , \text{ \hspace{1cm} Using S $\to$ $\epsilon$}\]

\underline{\textbf{Second Derivation:}}
\[ \underline{S} \to AS , \text{ \hspace{1cm} Using S $\to$ AS}\]
\[ \underline{A} S \to BAS , \text{ \hspace{1cm} Using A $\to$ BA}\]
\[ \underline{B}AS \to SBAS , \text{ \hspace{1cm} Using B $\to$ SB}\]
\[ \underline{S} BAS \to ASBAS , \text{ \hspace{1cm} Using S $\to$ AS}\]
\[ \underline{A} SBAS \to aSBAS , \text{ \hspace{1cm} Using A $\to$ a}\]
\[ a\underline{S}BAS \to aBAS , \text{ \hspace{1cm} Using S $\to$ $\epsilon$}\]
\[ a\underline{B}AS \to abAS , \text{ \hspace{1cm} Using B $\to$ b}\]
\[ ab\underline{A}S \to abBAS , \text{ \hspace{1cm} Using A $\to$ BA}\]
\[ ab\underline{B}AS \to abbAS , \text{ \hspace{1cm} Using B $\to$ b}\]
\[ abb\underline{A}S \to abbaS , \text{ \hspace{1cm} Using A $\to$ a}\]
\[ abba\underline{S} \to abba, \text{ \hspace{1cm} Using S $\to$ $\epsilon$}\]

Now, we have shown that there is a string $w = ``abba"$ that is derived ambiguously by the given CFG, so the given CFG is ambiguous. Hence Proved!
  \end{solution}
\end{questions}
\end{document}

%%% Local Variables:
%%% mode: latex
%%% TeX-master: t
%%% End:s
